ems/SimSTS2.v
@@ -1,0 +1,452 @@
+Require Import Coqlib.
+Require Import STS.
+Require Import Behavior.
+
+Set Implicit Arguments.
+
+Section BEHAVES.
+
+Variable L: semantics.
+
+Theorem of_state_ind2 :
+forall (P: _ -> _ -> Prop),
+(forall st0 retv, state_sort L st0 = final retv -> P st0 (Tr.done retv)) ->
+(forall st0, Beh.state_spin L st0 -> P st0 Tr.spin) ->
+(forall st0, P st0 Tr.nb) ->
+
+(forall st0 st1 ev evs
+ (SRT: state_sort L st0 = vis)
+ (STEP: _.(step) st0 (Some ev) st1)
+ (TL: Beh.of_state L st1 evs)
+  ,
+    P st0 (Tr.cons ev evs)) ->
+(forall st0 evs
+ (SRT: state_sort L st0 = demonic)
+ (STEP: Beh.union L st0
+   (fun e st1 =>
+    <<HD: e = None >> /\ <<TL: Beh.of_state L st1 evs >> /\ <<IH: P st1 evs>>)), P st0 evs) ->
+(forall st0 evs
+        (* (IH: forall st1 (STEP: L.(step) st0 None st1), P st1 evs) *)
+ (SRT: state_sort L st0 = angelic)
+ (STEP: Beh.inter L st0
+   (fun e st1 => <<HD: e = None >> /\ <<TL: Beh.of_state L st1 evs >> /\ <<IH: P st1 evs>>)),
+ P st0 evs) ->
+forall s t, Beh.of_state L s t -> P s t.
+Proof.
+  i. eapply Beh.of_state_ind; eauto.
+  { i. eapply H3; eauto.
+    unfold Beh.union in *. des. esplits; eauto.
+    pfold. eapply Beh.of_state_mon; eauto.
+  }
+  { i. eapply H4; eauto. ii. exploit STEP; eauto.
+    i. des. esplits; eauto.
+    pfold. eapply Beh.of_state_mon; eauto.
+  }
+  { punfold H5. eapply Beh.of_state_mon; eauto.
+    i. pclearbot. auto.
+  }
+Qed.
+
+Variant indC (of_state: L.(state) -> Tr.t -> Prop): L.(state) -> Tr.t -> Prop :=
+| indC_final
+    st0 retv
+    (FINAL: L.(state_sort) st0 = final retv)
+  :
+    indC of_state st0 (Tr.done retv)
+| indC_spin
+    st0
+    (SPIN: Beh.state_spin L st0)
+  :
+    indC of_state st0 (Tr.spin)
+| indC_nb
+    st0
+  :
+    indC of_state st0 (Tr.nb)
+| indC_vis
+    st0 st1 ev evs
+    (SRT: L.(state_sort) st0 = vis)
+    (STEP: _.(step) st0 (Some ev) st1)
+    (TL: of_state st1 evs)
+  :
+    indC of_state st0 (Tr.cons ev evs)
+| indC_demonic
+    st0
+    evs
+    (SRT: L.(state_sort) st0 = demonic)
+    (STEP: Beh.union L st0 (fun e st1 => (<<HD: e = None>>) /\ (<<TL: of_state st1 evs>>)))
+  :
+    indC of_state st0 evs
+| indC_angelic
+    st0
+    evs
+    (SRT: L.(state_sort) st0 = angelic)
+    (STEP: Beh.inter L st0 (fun e st1 => (<<HD: e = None>>) /\ (<<TL: of_state st1 evs>>)))
+  :
+    indC of_state st0 evs
+.
+
+Lemma indC_mon:
+  monotone2 indC.
+Proof.
+  ii. inv IN; eauto.
+  - econs 1; eauto.
+  - econs 2; eauto.
+  - econs 3; eauto.
+  - econs 4; eauto.
+  - econs 5; eauto. unfold Beh.union in *. des. esplits; eauto.
+  - econs 6; eauto. ii. exploit STEP; eauto. i. des. splits; auto.
+Qed.
+Hint Resolve indC_mon: paco.
+
+Lemma indC_spec:
+  indC <3= gupaco2 (Beh._of_state L) (cpn2 (Beh._of_state L)).
+Proof.
+  eapply wrespect2_uclo; eauto with paco.
+  econs; eauto with paco.
+  ii. inv PR.
+  { econs 1; eauto. }
+  { econs 2; eauto. }
+  { econs 3; eauto. }
+  { econs 4; eauto. eapply rclo2_base. auto. }
+  { econs 5; eauto. unfold Beh.union in *. des. esplits; eauto.
+    eapply Beh.of_state_mon; eauto. i. eapply rclo2_base. auto.
+  }
+  { econs 6; eauto. ii. exploit STEP; eauto. i. des. splits; auto.
+    eapply Beh.of_state_mon; eauto. i. eapply rclo2_base. auto.
+  }
+Qed.
+
+End BEHAVES.
+
+Lemma spin_nofinal
+      L st0
+      (SPIN: Beh.state_spin L st0)
+  :
+    forall retv, <<NOFIN: L.(state_sort) st0 <> final retv>>
+.
+Proof.
+  punfold SPIN. inv SPIN; ii; rewrite H in *; ss.
+Qed.
+
+Lemma spin_novis
+      L st0
+      (SPIN: Beh.state_spin L st0)
+  :
+    <<NOFIN: L.(state_sort) st0 <> vis>>
+.
+Proof.
+  punfold SPIN. inv SPIN; ii; rewrite H in *; ss.
+Qed.
+
+Lemma spin_astep
+      L st0 ev st1
+      (SRT: L.(state_sort) st0 = angelic)
+      (STEP: _.(step) st0 ev st1)
+      (SPIN: Beh.state_spin _ st0)
+  :
+    <<SPIN: Beh.state_spin _ st1>>
+.
+Proof.
+  exploit wf_angelic; et. i; clarify.
+  punfold SPIN. inv SPIN; rewrite SRT in *; ss.
+  exploit STEP0; et. i; des. pclearbot. et.
+Qed.
+
+
+
+Section SIM.
+
+  Variable L0 L1: semantics.
+
+  Inductive _sim (sim: bool -> bool -> L0.(state) -> L1.(state) -> Prop)
+            (i_src0: bool) (i_tgt0: bool) (st_src0: L0.(state)) (st_tgt0: L1.(state)): Prop :=
+  | sim_fin
+      retv
+      (SRT: _.(state_sort) st_src0 = final retv)
+      (SRT: _.(state_sort) st_tgt0 = final retv)
+    :
+      _sim sim i_src0 i_tgt0 st_src0 st_tgt0
+  | sim_demonic_src
+      (SRT: _.(state_sort) st_src0 = demonic)
+      (SIM: exists st_src1
+                   (STEP: _.(step) st_src0 None st_src1)
+        ,
+          exists i_src1, <<SIM: _sim sim i_src1 i_tgt0 st_src1 st_tgt0>>)
+    :
+      _sim sim i_src0 i_tgt0 st_src0 st_tgt0
+  | sim_demonic_tgt
+      (SRT: _.(state_sort) st_tgt0 = demonic)
+      (* (FIN: _.(state_sort) st_src0 = final <-> _.(state_sort) st_tgt0 = final) *)
+      (SIM: forall st_tgt1
+                   (STEP: _.(step) st_tgt0 None st_tgt1)
+        ,
+          exists i_tgt1, <<SIM: _sim sim i_src0 i_tgt1 st_src0 st_tgt1>>)
+    :
+      _sim sim i_src0 i_tgt0 st_src0 st_tgt0
+  | sim_progress
+      (SIM: sim false false st_src0 st_tgt0)
+      (SRC: i_src0 = true)
+      (TGT: i_tgt0 = true)
+    :
+      _sim sim i_src0 i_tgt0 st_src0 st_tgt0
+  .
+
+  Lemma _sim_ind2 sim (P: bool -> bool -> L0.(state) -> L1.(state) -> Prop)
+        (FIN: forall
+            i_src0 i_tgt0 st_src0 st_tgt0
+            retv
+            (SRT: _.(state_sort) st_src0 = final retv)
+            (SRT: _.(state_sort) st_tgt0 = final retv),
+            P i_src0 i_tgt0 st_src0 st_tgt0)
+        (DMSRC: forall
+            i_src0 i_tgt0 st_src0 st_tgt0
+            (SRT: _.(state_sort) st_src0 = demonic)
+            (SIM: exists st_src1
+                         (STEP: _.(step) st_src0 None st_src1)
+              ,
+                exists i_src1, <<SIM: _sim sim i_src1 i_tgt0 st_src1 st_tgt0>> /\ <<IH: P i_src1 i_tgt0 st_src1 st_tgt0>>),
+            P i_src0 i_tgt0 st_src0 st_tgt0)
+        (DMTGT: forall
+            i_src0 i_tgt0 st_src0 st_tgt0
+            (SRT: _.(state_sort) st_tgt0 = demonic)
+            (SIM: forall st_tgt1
+                         (STEP: _.(step) st_tgt0 None st_tgt1)
+              ,
+                exists i_tgt1, <<SIM: _sim sim i_src0 i_tgt1 st_src0 st_tgt1>> /\ <<IH: P i_src0 i_tgt1 st_src0 st_tgt1>>),
+            P i_src0 i_tgt0 st_src0 st_tgt0)
+        (PROGRESS:
+           forall
+             i_src0 i_tgt0 st_src0 st_tgt0
+             (SIM: sim false false st_src0 st_tgt0)
+             (SRC: i_src0 = true)
+             (TGT: i_tgt0 = true),
+             P i_src0 i_tgt0 st_src0 st_tgt0)
+    :
+      forall i_src0 i_tgt0 st_src0 st_tgt0
+             (SIM: _sim sim i_src0 i_tgt0 st_src0 st_tgt0),
+        P i_src0 i_tgt0 st_src0 st_tgt0.
+  Proof.
+    fix IH 5. i. inv SIM.
+    { eapply FIN; eauto. }
+    { eapply DMSRC; eauto.
+      des. esplits; eauto. }
+    { eapply DMTGT; eauto. i.
+      hexploit SIM0; eauto. i. des. esplits; eauto. }
+    { eapply PROGRESS; eauto. }
+  Qed.
+
+  Lemma sim_mon: monotone4 _sim.
+  Proof.
+    ii. revert x0 x1 x2 x3 IN. eapply _sim_ind2; i; clarify.
+    { econs 1; eauto. }
+    { econs 2; eauto. des. esplits; eauto. }
+    { econs 3; eauto. i. hexploit SIM; eauto. i. des. esplits; eauto. }
+    { econs 4; eauto. }
+  Qed.
+
+  Definition sim: _ -> _ -> _ -> _ -> Prop := paco4 _sim bot4.
+
+  Hint Constructors _sim.
+  Hint Unfold sim.
+  Hint Resolve sim_mon: paco.
+
+  Lemma sim_ind (P: bool -> bool -> L0.(state) -> L1.(state) -> Prop)
+        (FIN: forall
+            i_src0 i_tgt0 st_src0 st_tgt0
+            retv
+            (SRT: _.(state_sort) st_src0 = final retv)
+            (SRT: _.(state_sort) st_tgt0 = final retv),
+            P i_src0 i_tgt0 st_src0 st_tgt0)
+        (DMSRC: forall
+            i_src0 i_tgt0 st_src0 st_tgt0
+            (SRT: _.(state_sort) st_src0 = demonic)
+            (SIM: exists st_src1
+                         (STEP: _.(step) st_src0 None st_src1)
+              ,
+                exists i_src1, <<SIM: sim i_src1 i_tgt0 st_src1 st_tgt0>> /\ <<IH: P i_src1 i_tgt0 st_src1 st_tgt0>>),
+            P i_src0 i_tgt0 st_src0 st_tgt0)
+        (DMTGT: forall
+            i_src0 i_tgt0 st_src0 st_tgt0
+            (SRT: _.(state_sort) st_tgt0 = demonic)
+            (SIM: forall st_tgt1
+                         (STEP: _.(step) st_tgt0 None st_tgt1)
+              ,
+                exists i_tgt1, <<SIM: sim i_src0 i_tgt1 st_src0 st_tgt1>> /\ <<IH: P i_src0 i_tgt1 st_src0 st_tgt1>>),
+            P i_src0 i_tgt0 st_src0 st_tgt0)
+        (PROGRESS:
+           forall
+             i_src0 i_tgt0 st_src0 st_tgt0
+             (SIM: sim false false st_src0 st_tgt0)
+             (SRC: i_src0 = true)
+             (TGT: i_tgt0 = true),
+             P i_src0 i_tgt0 st_src0 st_tgt0)
+    :
+      forall i_src0 i_tgt0 st_src0 st_tgt0
+             (SIM: sim i_src0 i_tgt0 st_src0 st_tgt0),
+        P i_src0 i_tgt0 st_src0 st_tgt0.
+  Proof.
+    i. eapply (@_sim_ind2 sim P); eauto.
+    { i. eapply DMSRC; eauto. des. esplits; eauto.
+      pfold. eapply sim_mon; eauto.
+    }
+    { i. eapply DMTGT; eauto. i. hexploit SIM0; eauto. i. des. esplits; eauto.
+      pfold. eapply sim_mon; eauto.
+    }
+    { punfold SIM. eapply sim_mon; eauto. i. pclearbot. auto. }
+  Qed.
+
+  Record simulation: Prop := mk_simulation {
+    sim_init: exists i_src0 i_tgt0, <<SIM: sim i_src0 i_tgt0 L0.(initial_state) L1.(initial_state)>>;
+  }
+  .
+
+  Lemma admitt: False. Admitted.
+  Ltac admitt := exfalso; apply admitt.
+
+  Ltac pc H := rr in H; desH H; ss.
+  Lemma adequacy_spin
+        i_src0 i_tgt0 st_src0 st_tgt0
+        (SIM: sim i_src0 i_tgt0 st_src0 st_tgt0)
+        (SPIN: Beh.state_spin L1 st_tgt0)
+    :
+      <<SPIN: Beh.state_spin L0 st_src0>>
+  .
+  Proof.
+    ginit.
+    { i. eapply cpn1_wcompat; eauto. eapply Beh.state_spin_mon. }
+    revert i_src0 i_tgt0 st_src0 st_tgt0 SIM SPIN. gcofix CIH.
+    intros ? ? ? ? SIM. induction SIM using sim_ind; i; clarify.
+    - (** final **)
+      exfalso. punfold SPIN. inv SPIN; rewrite SRT0 in *; ss.
+    - (** dsrc **)
+      des. gstep. econs 2; eauto. esplits; eauto.
+      eapply gpaco1_mon; eauto. ss.
+    - (** dtgt **)
+      punfold SPIN. inv SPIN; rewrite SRT in *; ss. des. pclearbot.
+      exploit wf_demonic; et; i; clarify.
+      exploit SIM; et. i; des. eapply IH; eauto.
+    - (** progress **)
+      remember false in SIM at 1.
+      remember false in SIM at 1.
+      revert Heqb. clear Heqb0. revert SPIN.
+      induction SIM using sim_ind; i; clarify.
+      + exfalso. punfold SPIN. inv SPIN; rewrite SRT1 in *; clarify.
+      + des. gstep. econs 2; auto. esplits; eauto.
+        gbase. eapply CIH; eauto.
+      + punfold SPIN. inv SPIN; rewrite SRT in *; clarify. des.
+        exploit wf_demonic; et; i; clarify. pclearbot.
+        exploit SIM; et. i; des. eapply IH; eauto.
+  Qed.
+
+  Lemma adequacy_aux
+        i_src0 i_tgt0 st_src0 st_tgt0
+        (SIM: sim i_src0 i_tgt0 st_src0 st_tgt0)
+    :
+      <<IMPR: Beh.improves (Beh.of_state L0 st_src0) (Beh.of_state L1 st_tgt0)>>
+  .
+  Proof.
+    ginit.
+    { i. eapply cpn2_wcompat; eauto. eapply Beh.of_state_mon. }
+    revert i_tgt0 i_src0 st_src0 st_tgt0 SIM. gcofix CIH.
+    i. rename x2 into tr.
+    punfold PR. revert i_src0 i_tgt0 st_src0 SIM.
+    induction PR using Beh.of_state_ind; ii; ss; rename st0 into st_tgt0.
+    - (** done **)
+      revert retv H.
+      induction SIM using sim_ind; i; clarify.
+      + rewrite SRT0 in *. clarify. gstep. econs; eauto.
+      + des. guclo indC_spec. econs 5; eauto. red. esplits; eauto.
+      + rewrite SRT in *. clarify.
+      + admitt.
+    - (** spin **)
+      exploit adequacy_spin; eauto. i.
+      gstep. econs. et.
+    - (** nb **)
+      gstep. econs; eauto.
+    - (** cons **)
+      pc TL. induction SIM using sim_ind; i; try rewrite SRT in *; clarify.
+      + (** d_ **)
+        des. guclo indC_spec. econs 5; eauto. red. esplits; eauto.
+      + (** progress **)
+        remember false in SIM at 1.
+        remember false in SIM at 1.
+        clear Heqb0. revert Heqb.
+        revert ev SRT STEP.
+        induction SIM using sim_ind; i; try rewrite SRT0 in *; clarify.
+        * des. guclo indC_spec. econs 5; eauto. red. esplits; eauto.
+
+          exploit IH; eauto. i.
+          guclo indC_spec. econs 5; eauto. red. esplits; eauto.
+        *
+
+
+          rewrite SRT0 in *. clarify.
+        * rewrite SRT0 in *. clarify.
+        * rewrite SRT0 in *. clarify.
+
+
+        punfold SIM. induction SIM with
+
+                       inv SIM; try rewrite SRT in *; clarify.
+        des.
+
+
+        eapply IH; eauto.
+        guclo Beh.dstep_clo_spec. econs; eauto.
+      + (** a_ **)
+        guclo Beh.astep_clo_spec. econs; eauto. ii.
+        exploit SIM0; et. i. des. pc SIM. et.
+
+      revert i_src0 st_src0 SIM.
+      induction (WFTGT i_tgt0).
+      clear H. rename x into i_tgt0. rename H0 into IHTGT. i.
+      pc TL. punfold SIM. inv SIM; try rewrite SRT in *; ss.
+      + (** vv **)
+        specialize (SIM0 ev st1). apply SIM0 in STEP; clear SIM0; des.
+        gstep. econs 4; eauto. pc SIM. gbase. eapply CIH; eauto.
+      + (** vis stuck **)
+        apply STUCK in STEP. clarify.
+      + (** d_ **)
+        des. pc SIM.
+        guclo Beh.dstep_clo_spec. econs; eauto.
+      + (** a_ **)
+        guclo Beh.astep_clo_spec. econs; eauto. ii.
+        exploit SIM0; et. i. des. pc SIM. et.
+    - (** demonic **)
+      revert i_src0 st_src0 SIM.
+      induction (WFTGT i_tgt0).
+      clear H. rename x into i_tgt0. rename H0 into IHTGT. i.
+      rr in STEP. des. clarify. rename st1 into st_tgt1.
+      punfold SIM. inv SIM; try rewrite SRT in *; ss.
+      + des. pc SIM.
+        guclo Beh.dstep_clo_spec. econs; et.
+      + exploit SIM0; et. i. des. pc SIM.
+        eapply IH; et.
+      + guclo Beh.astep_clo_spec. econs; et. ii.
+        exploit SIM0; et. i. des. pc SIM. et.
+    - (** angelic **)
+      revert i_src0 st_src0 SIM.
+      induction (WFTGT i_tgt0).
+      clear H. rename x into i_tgt0. rename H0 into IHTGT. i.
+      punfold SIM. inv SIM; try rewrite SRT in *; ss.
+      + des. pc SIM.
+        guclo Beh.dstep_clo_spec. econs; et.
+      + guclo Beh.astep_clo_spec. econs; et. ii.
+        exploit SIM0; et. i. des. pc SIM. et.
+      + des. pc SIM. exploit STEP; et. i. des. et.
+  Qed.
+
+  Theorem adequacy
+          (SIM: simulation)
+    :
+      <<IMPR: Beh.improves (Beh.of_program L0) (Beh.of_program L1)>>
+  .
+  Proof.
+    inv SIM. des.
+    eapply adequacy_aux; et.
+  Qed.
+
+End SIM.
+Hint Constructors _sim.
+Hint Unfold sim.
+Hint Resolve sim_mon: paco.
